WIP

security/MemoryDelta.v
@@ -3,6 +3,156 @@ Require Import Coqlib Maps Errors Integers Values Memory Globalenvs.
 Require Import AST Linking Smallstep Events Behaviors.
 Require Import MemoryWeak.
 
+
+
+Section AUX.
+
+  Lemma alloc_left_unmapped_winject_keep:
+    forall f m1 m2 c lo hi m1' b1,
+      winject f m1 m2 ->
+      Mem.alloc m1 c lo hi = (m1', b1) ->
+      winject f m1' m2.
+  Proof.
+    intros. set (f' := fun b => if eq_block b b1 then None else f b).
+    cut (winject f' m1' m2 /\ inject_incr f f' /\ f' b1 = None /\ (forall b, b <> b1 -> f' b = f b)).
+    { clear - f'. intros (INJ & INCR & _ & _). unfold inject_incr in INCR.
+      assert (f' = f).
+      { eapply Axioms.functional_extensionality. intros x. destruct (eq_block x b1).
+        - subst x. destruct (f b1) eqn:FB.
+          + destruct p. specialize (INCR _ _ _ FB). auto.
+          + subst f'. simpl. rewrite pred_dec_true; auto.
+        - subst f'. simpl. rewrite pred_dec_false; auto.
+      }
+      rewrite <- H. apply INJ.
+    }
+    inversion H. assert (inject_incr f f').
+    red; unfold f'; intros. destruct (eq_block b b1). subst b.
+    assert (f b1 = None). eauto with mem. congruence.
+    auto.
+    assert (mem_winj f' m1 m2).
+    inversion mwi_inj; constructor; eauto with mem.
+    unfold f'; intros. destruct (eq_block b0 b1). congruence. eauto.
+    unfold f'; intros. destruct (eq_block b0 b1). congruence. eauto.
+    unfold f'; intros. destruct (eq_block b0 b1). congruence.
+    unfold f'; intros. destruct (eq_block b0 b1). congruence.
+    eapply mwi_align; eauto.
+    split. constructor.
+    (* inj *)
+    eapply alloc_left_unmapped_winj; eauto. unfold f'; apply dec_eq_true.
+    (* freeblocks *)
+    intros. unfold f'. destruct (eq_block b b1). auto.
+    apply mi_freeblocks. red; intro; elim H3. eauto with mem.
+    (* mappedblocks *)
+    unfold f'; intros. destruct (eq_block b b1). congruence. eauto.
+    (* no overlap *)
+    unfold f'; red; intros.
+    destruct (eq_block b0 b1); destruct (eq_block b2 b1); try congruence.
+    eapply mwi_no_overlap. eexact H3. eauto. eauto.
+    exploit Mem.perm_alloc_inv. eauto. eexact H6. rewrite dec_eq_false; auto.
+    exploit Mem.perm_alloc_inv. eauto. eexact H7. rewrite dec_eq_false; auto.
+    (* representable *)
+    unfold f'; intros.
+    destruct (eq_block b b1); try discriminate.
+    eapply mwi_representable; try eassumption.
+    destruct H4; eauto using Mem.perm_alloc_4.
+    (* perm inv *)
+    intros. unfold f' in H3; destruct (eq_block b0 b1); try discriminate.
+    exploit mwi_perm_inv; eauto.
+    intuition eauto using Mem.perm_alloc_1, Mem.perm_alloc_4.
+    (* incr *)
+    split. auto.
+    (* image *)
+    split. unfold f'; apply dec_eq_true.
+    (* incr *)
+    intros; unfold f'; apply dec_eq_false; auto.
+  Qed.
+
+  Lemma alloc_left_unmapped_inject_keep:
+    forall f m1 m2 c lo hi m1' b1,
+      Mem.inject f m1 m2 ->
+      Mem.alloc m1 c lo hi = (m1', b1) ->
+      Mem.inject f m1' m2.
+  Proof.
+    intros. set (f' := fun b => if eq_block b b1 then None else f b).
+    cut (Mem.inject f' m1' m2 /\ inject_incr f f' /\ f' b1 = None /\ (forall b, b <> b1 -> f' b = f b)).
+    { clear - f'. intros (INJ & INCR & _ & _). unfold inject_incr in INCR.
+      assert (f' = f).
+      { eapply Axioms.functional_extensionality. intros x. destruct (eq_block x b1).
+        - subst x. destruct (f b1) eqn:FB.
+          + destruct p. specialize (INCR _ _ _ FB). auto.
+          + subst f'. simpl. rewrite pred_dec_true; auto.
+        - subst f'. simpl. rewrite pred_dec_false; auto.
+      }
+      rewrite <- H. apply INJ.
+    }
+    inversion H. assert (inject_incr f f').
+    red; unfold f'; intros. destruct (eq_block b b1). subst b.
+    assert (f b1 = None). eauto with mem. congruence.
+    auto.
+    assert (Mem.mem_inj f' m1 m2).
+    inversion mi_inj; constructor; eauto with mem.
+    unfold f'; intros. destruct (eq_block b0 b1). congruence. eauto.
+    unfold f'; intros. destruct (eq_block b0 b1). congruence. eauto.
+    unfold f'; intros. destruct (eq_block b0 b1). congruence.
+    unfold f'; intros. destruct (eq_block b0 b1). congruence.
+    eapply mi_align; eauto.
+    unfold f'; intros. destruct (eq_block b0 b1). congruence.
+    apply memval_inject_incr with f; auto.
+    split. constructor.
+    (* inj *)
+    eapply Mem.alloc_left_unmapped_inj; eauto. unfold f'; apply dec_eq_true.
+    (* freeblocks *)
+    intros. unfold f'. destruct (eq_block b b1). auto.
+    apply mi_freeblocks. red; intro; elim H3. eauto with mem.
+    (* mappedblocks *)
+    unfold f'; intros. destruct (eq_block b b1). congruence. eauto.
+    (* no overlap *)
+    unfold f'; red; intros.
+    destruct (eq_block b0 b1); destruct (eq_block b2 b1); try congruence.
+    eapply mi_no_overlap. eexact H3. eauto. eauto.
+    exploit Mem.perm_alloc_inv. eauto. eexact H6. rewrite dec_eq_false; auto.
+    exploit Mem.perm_alloc_inv. eauto. eexact H7. rewrite dec_eq_false; auto.
+    (* representable *)
+    unfold f'; intros.
+    destruct (eq_block b b1); try discriminate.
+    eapply mi_representable; try eassumption.
+    destruct H4; eauto using Mem.perm_alloc_4.
+    (* perm inv *)
+    intros. unfold f' in H3; destruct (eq_block b0 b1); try discriminate.
+    exploit mi_perm_inv; eauto.
+    intuition eauto using Mem.perm_alloc_1, Mem.perm_alloc_4.
+    (* incr *)
+    split. auto.
+    (* image *)
+    split. unfold f'; apply dec_eq_true.
+    (* incr *)
+    intros; unfold f'; apply dec_eq_false; auto.
+  Qed.
+
+End AUX.
+
+
+Section PUBINJ.
+
+  (* Memory injection for public global symbols: visible for external calls *)
+  Definition meminj_public (ge: Senv.t): meminj :=
+    fun b => match Senv.invert_symbol ge b with
+          | Some id => if Senv.public_symbol ge id then Some (b, 0%Z) else None
+          | None => None
+          end.
+
+  Definition meminj_strict (j: meminj) := forall b1 b2 b' ofsd1 ofsd2, j b1 = Some (b', ofsd1) -> j b2 = Some (b', ofsd2) -> b1 = b2.
+
+  Lemma meminj_public_strict ge: meminj_strict (meminj_public ge).
+  Proof.
+    unfold meminj_strict. intros. unfold meminj_public in *; simpl in *.
+    destruct (Senv.invert_symbol ge b1) eqn:INV1. 2: congruence. destruct (Senv.public_symbol ge i) eqn:PUB1. 2: congruence. inv H.
+    destruct (Senv.invert_symbol ge b2) eqn:INV2. 2: congruence. destruct (Senv.public_symbol ge i0) eqn:PUB2. 2: congruence. inv H0.
+    auto.
+  Qed.
+
+End PUBINJ.
+
 Section MEMDELTA.
 
   (** Memory delta data and apply *)
@@ -139,6 +289,13 @@ Section MEMDELTA.
     destruct a; [rewrite mem_delta_apply_store_none | rewrite mem_delta_apply_bytes_none | rewrite mem_delta_apply_alloc_none | rewrite mem_delta_apply_free_none]; rewrite IHd; auto.
   Qed.
 
+  Lemma mem_delta_apply_some
+        d om m'
+        (APPD: mem_delta_apply d om = Some m')
+    :
+    exists m, om = Some m.
+  Proof. destruct om; eauto. rewrite mem_delta_apply_none in APPD. inv APPD. Qed.    
+
   (* Lemma mem_delta_apply_eq *)
   (*       d m0 *)
   (*   : *)
@@ -221,6 +378,13 @@ Section MEMDELTA.
     induction d; auto. rewrite mem_delta_apply_inj_cons.
     destruct a. destruct d0 as [[[[a0 a1] a2] a3] a4]. destruct (j a1). destruct p. rewrite mem_delta_apply_store_none. all: rewrite IHd; auto.
   Qed.
+
+  Lemma mem_delta_apply_inj_some
+        j d om m'
+        (APPD: mem_delta_apply_inj j d om = Some m')
+    :
+    exists m, om = Some m.
+  Proof. destruct om; eauto. rewrite mem_delta_apply_inj_none in APPD. inv APPD. Qed.    
 
   (* Lemma mem_delta_apply_inj_eq *)
   (*       j d m0 *)
@@ -378,13 +542,46 @@ Section MEMDELTA.
       }
   Qed.
 
+  Lemma mem_delta_inj_unchanged_on
+        j d m m'
+        (STRICT: meminj_strict j)
+        (APPD: mem_delta_apply_inj j d (Some m) = Some m')
+    :
+    Mem.unchanged_on (fun b ofs => (forall b0 ofsd, j b0 <> Some (b, ofsd)) \/ (exists b0 ofsd, j b0 = Some (b, ofsd) /\ mem_delta_unchanged d b0 (ofs - ofsd))) m m'.
+  Proof.
+    revert m m' APPD. induction d; intros; simpl.
+    { simpl in APPD. inv APPD. apply Mem.unchanged_on_refl. }
+    rewrite mem_delta_apply_inj_cons in APPD. destruct a.
+    - destruct d0 as [[[[ch b] ofs] v] cp]. destruct (j b) as [[b' ofs'] |] eqn:JB.
+      + exploit mem_delta_apply_inj_some. eauto. intros (mi & MEM). rewrite MEM in APPD.
+        specialize (IHd _ _ APPD). eapply Mem.unchanged_on_trans.
+        2:{ eapply Mem.unchanged_on_implies. eapply IHd. intros. simpl. inv H; eauto. destruct H1 as (b1 & ofsd & JB1 & UNCHG). inv UNCHG. right. eauto. }
+        { simpl in *. eapply Mem.store_unchanged_on. eauto. intros. intros [CC | CC].
+          - specialize (CC b ofs'). congruence.
+          - destruct CC as (b1 & ofsd & JB1 & UNCHG). inv UNCHG. simpl in H2. destruct (Pos.eqb_spec b b1).
+            + subst b1. rewrite JB in JB1. inv JB1. specialize (H2 eq_refl). lia.
+            + specialize (STRICT _ _ _ _ _ JB JB1). subst b1. lia.
+        }
+      + specialize (IHd _ _ APPD). eapply Mem.unchanged_on_implies. eapply IHd. intros. simpl. inv H; eauto. destruct H1 as (b1 & ofsd & JB1 & UNCHG). inv UNCHG. right. eauto.
+    - specialize (IHd _ _ APPD). eapply Mem.unchanged_on_implies. eapply IHd. intros. simpl. inv H; eauto. destruct H1 as (b1 & ofsd & JB1 & UNCHG). inv UNCHG. right. eauto.
+    - specialize (IHd _ _ APPD). eapply Mem.unchanged_on_implies. eapply IHd. intros. simpl. inv H; eauto. destruct H1 as (b1 & ofsd & JB1 & UNCHG). inv UNCHG. right. eauto.
+    - specialize (IHd _ _ APPD). eapply Mem.unchanged_on_implies. eapply IHd. intros. simpl. inv H; eauto. destruct H1 as (b1 & ofsd & JB1 & UNCHG). inv UNCHG. right. eauto.
+  Qed.
 
-  (* Lemma nth_of_encode_val *)
-  (*       ch v ofs ofs' *)
-  (*       (GE: ofs <= ofs' < ofs + (size_chunk ch)) *)
-  (*   : *)
-  (*   exists mv, nth_error (encode_val ch v) (Z.to_nat (ofs' - ofs)) = Some mv. *)
-  (* Proof. *)
+
+  Lemma get_from_setN_same_upto_ofs
+        ofs0 ofs l ofsd
+        (OFS: ofs0 <= ofs < ofs0 + Z.of_nat (Datatypes.length l))
+        (mc1 mc2 : (ZMap.t memval))
+    :
+    ZMap.get ofs (Mem.setN l ofs0 mc1) = ZMap.get (ofs + ofsd) (Mem.setN l (ofs0 + ofsd) mc2).
+  Proof.
+    revert ofs0 ofs ofsd OFS mc1 mc2. induction l; simpl; intros.
+    { lia. }
+    destruct (Z.eqb_spec ofs0 ofs).
+    { subst ofs0. clear OFS. rewrite ! Mem.setN_outside; try lia. rewrite ! ZMap.gss. auto. }
+    { replace (ofs0 + ofsd + 1) with ((ofs0 + 1) + ofsd) by lia. eapply IHl. lia. }
+  Qed.
 
   Lemma get_from_setN_same
         ofs0 ofs l
@@ -393,12 +590,23 @@ Section MEMDELTA.
     :
     ZMap.get ofs (Mem.setN l ofs0 mc1) = ZMap.get ofs (Mem.setN l ofs0 mc2).
   Proof.
-    revert ofs0 ofs OFS mc1 mc2. induction l; simpl; intros.
-    { lia. }
-    destruct (Z.eqb_spec ofs0 ofs).
-    { subst ofs0. clear OFS. rewrite ! Mem.setN_outside; try lia. rewrite ! ZMap.gss. auto. }
-    { eapply IHl. lia. }
+    replace ofs with (ofs + 0) at 2 by lia. replace ofs0 with (ofs0 + 0) at 2 by lia. eapply get_from_setN_same_upto_ofs; auto.
   Qed.
+
+  Lemma mem_store_same_upto_ofs
+        ofs ofs0 ch0 v0 cp0 ofsd b b' m1 m2 m1' m2'
+        (OFS: ofs0 <= ofs < ofs0 + size_chunk ch0)
+        (MEM1: Mem.store ch0 m1 b ofs0 v0 cp0 = Some m1')
+        (MEM2: Mem.store ch0 m2 b' (ofs0 + ofsd) v0 cp0 = Some m2')
+    :
+    ZMap.get ofs (Mem.mem_contents m1') !! b = ZMap.get (ofs + ofsd) (Mem.mem_contents m2') !! b'.
+  Proof.
+    apply Mem.store_mem_contents in MEM1, MEM2. rewrite MEM1, MEM2. rewrite ! PMap.gss.
+    rewrite size_chunk_conv, <- (encode_val_length ch0 v0) in OFS.
+    remember (encode_val ch0 v0) as l. remember (Mem.mem_contents m1) as mc1. remember (Mem.mem_contents m2) as mc2. clear - OFS.
+    eapply get_from_setN_same_upto_ofs. auto.
+  Qed.
+
 
   Definition mem_delta_changed_store (d: mem_delta_store) (b': block) (ofs': Z): Prop :=
     let '(ch, b, ofs, v, cp) := d in
@@ -414,10 +622,8 @@ Section MEMDELTA.
     ZMap.get ofs (Mem.mem_contents m1') !! b = ZMap.get ofs (Mem.mem_contents m2') !! b.
   Proof.
     destruct d as [[[[ch0 b0] ofs0] v0] cp0]. destruct CHG as (BLK & OFS). subst b0.
-    simpl in *. apply Mem.store_mem_contents in APPD1, APPD2. rewrite APPD1, APPD2. rewrite ! PMap.gss.
-    rewrite size_chunk_conv, <- (encode_val_length ch0 v0) in OFS.
-    remember (encode_val ch0 v0) as l. remember (Mem.mem_contents m1) as mc1. remember (Mem.mem_contents m2) as mc2. clear - OFS.
-    eapply get_from_setN_same. auto.
+    simpl in *. replace ofs with (ofs + 0) at 2 by lia. eapply mem_store_same_upto_ofs; eauto.
+    replace (ofs0 + 0) with ofs0 by lia. eauto.
   Qed.
 
   Definition mem_delta_changed_bytes (d: mem_delta_bytes) (b': block) (ofs': Z): Prop :=
@@ -469,202 +675,255 @@ Section MEMDELTA.
   Definition mem_delta_changed (d: mem_delta) (b: block) (ofs: Z) :=
     Exists (fun k => mem_delta_kind_changed k b ofs) d.
 
-  Definition mem_delta_kind_changed_by_store_inj (j: meminj) (k: mem_delta_kind) (b: block) (ofs: Z) :=
-    match k with
-    | mem_delta_kind_store (ch0, b0, ofs0, v0, cp0) =>
-        match j b0 with
-        | Some _ => mem_delta_changed_store (ch0, b0, ofs0, v0, cp0) b ofs
-        | _ => False
-        end
-    | _ => False
-    end.
+  (* Definition mem_delta_kind_changed_by_store_inj (j: meminj) (k: mem_delta_kind) (b: block) (ofs: Z) := *)
+  (*   match k with *)
+  (*   | mem_delta_kind_store (ch0, b0, ofs0, v0, cp0) => *)
+  (*       match j b0 with *)
+  (*       | Some _ => mem_delta_changed_store (ch0, b0, ofs0, v0, cp0) b ofs *)
+  (*       | _ => False *)
+  (*       end *)
+  (*   | _ => False *)
+  (*   end. *)
 
-  Definition mem_delta_changed_by_store_inj (j: meminj) (d: mem_delta) (b: block) (ofs: Z) :=
-    Exists (fun k => mem_delta_kind_changed_by_store_inj j k b ofs) d.
+  (* Definition mem_delta_changed_by_store_inj (j: meminj) (d: mem_delta) (b: block) (ofs: Z) := *)
+  (*   Exists (fun k => mem_delta_kind_changed_by_store_inj j k b ofs) d. *)
 
-  Lemma mem_delta_changed_only_by_store
-        j d b ofs
-        (INJ: j b <> None)
-        (CHG: mem_delta_changed d b ofs)
-        (WF: mem_delta_inj_wf j d)
+  (** Propperties *)
+  Lemma mem_delta_cases_store
+        d b ofs
     :
-    mem_delta_changed_by_store_inj j d b ofs.
-  Proof.
+    mem_delta_unchanged_store d b ofs \/ mem_delta_changed_store d b ofs.
+  Proof. destruct d as [[[[ch0 b0] ofs0] v0] cp0]. simpl. lia. Qed.
 
-  Abort.
+  Lemma mem_delta_cases_bytes
+        d b ofs
+    :
+    mem_delta_unchanged_bytes d b ofs \/ mem_delta_changed_bytes d b ofs.
+  Proof. destruct d as [[[b0 ofs0] mvs] cp0]. simpl. lia. Qed.
+
+  Lemma mem_delta_cases_alloc
+        d b ofs
+    :
+    mem_delta_unchanged_alloc d b ofs \/ mem_delta_changed_alloc d b ofs.
+  Proof. destruct d as [[x y] z]. simpl. auto. Qed.
+
+  Lemma mem_delta_cases_free
+        d b ofs
+    :
+    mem_delta_unchanged_free d b ofs \/ mem_delta_changed_free d b ofs.
+  Proof. destruct d as [[[b0 lo] hi] cp0]. simpl. lia. Qed.
+
+  Lemma mem_delta_cases_kind
+        d b ofs
+    :
+    mem_delta_kind_unchanged d b ofs \/ mem_delta_kind_changed d b ofs.
+  Proof. destruct d; simpl. apply mem_delta_cases_store. apply mem_delta_cases_bytes. apply mem_delta_cases_alloc. apply mem_delta_cases_free. Qed.
 
   Lemma mem_delta_unchanged_or_changed
         d b ofs
     :
     mem_delta_unchanged d b ofs \/ mem_delta_changed d b ofs.
   Proof.
-  Abort.
+    induction d.
+    { left. constructor 1. }
+    destruct IHd.
+    2:{ right. constructor 2. auto. }
+    destruct (mem_delta_cases_kind a b ofs).
+    - left. constructor; auto.
+    - right. constructor 1; auto.
+  Qed.
+
+  Lemma mem_delta_changed_only_by_store
+        j d b ofs
+        (STRICT: meminj_strict j)
+        b' ofsd
+        (INJ: j b = Some (b', ofsd))
+        (WF: mem_delta_inj_wf j d)
+        (CHG: mem_delta_changed d b ofs)
+        m1 m1' m2 m2'
+        (PERM1: Mem.perm m1 b ofs Cur Readable)
+        (PERM2: Mem.perm m2 b' (ofs + ofsd) Cur Readable)
+        (APPD1: mem_delta_apply d (Some m1) = Some m1')
+        (APPD2: mem_delta_apply_inj j d (Some m2) = Some m2')
+    :
+    ZMap.get ofs (Mem.mem_contents m1') !! b = ZMap.get (ofs + ofsd) (Mem.mem_contents m2') !! b'.
+  Proof.
+    revert WF CHG m1 m1' m2 m2' PERM1 PERM2 APPD1 APPD2. induction d; intros.
+    { inv CHG. }
+    rewrite mem_delta_apply_cons in APPD1. rewrite mem_delta_apply_inj_cons in APPD2. inv WF. rename H1 into WF1, H2 into WF2. inv CHG.
+    2:{ specialize (IHd WF2 H0). destruct a.
+        - destruct d0 as [[[[ch0 b0 ]ofs0] v0] cp0]. destruct (j b0) as [[b0' ofs0'] |] eqn:JB.
+          + exploit mem_delta_apply_some. eapply APPD1. intros (mi1 & MEM1). rewrite MEM1 in APPD1.
+            exploit mem_delta_apply_inj_some. eapply APPD2. intros (mi2 & MEM2). rewrite MEM2 in APPD2.
+            simpl in *. eapply IHd. 3,4: eauto. 1,2: eapply Mem.perm_store_1; eauto.
+          + exploit mem_delta_apply_some. eapply APPD1. intros (mi1 & MEM1). rewrite MEM1 in APPD1. simpl in *. eapply IHd. 3,4: eauto. all: auto. eapply Mem.perm_store_1; eauto.
+        - exploit mem_delta_apply_some. eapply APPD1. intros (mi1 & MEM1). rewrite MEM1 in APPD1. destruct d0 as [[[w x] y] z]. simpl in *. eapply IHd. 3,4: eauto. all: auto.
+          eapply Mem.perm_storebytes_1; eauto.
+        - exploit mem_delta_apply_some. eapply APPD1. intros (mi1 & MEM1). rewrite MEM1 in APPD1. destruct d0 as [[x y] z]. simpl in *. eapply IHd. 3,4: eauto. all: auto.
+          destruct (Mem.alloc m1 x y z) eqn:ALLOC. simpl in MEM1. inv MEM1. eapply Mem.perm_alloc_1; eauto.
+        - exploit mem_delta_apply_some. eapply APPD1. intros (mi1 & MEM1). rewrite MEM1 in APPD1. destruct d0 as [[[w x] y] z]. simpl in *. eapply IHd. 3,4: eauto. all: auto.
+          eapply Mem.perm_free_1; eauto. left. intros CC. subst. congruence.
+    }
+    rename H0 into CHG. destruct (mem_delta_unchanged_or_changed d b ofs).
+    2:{ specialize (IHd WF2 H). destruct a.
+        - destruct d0 as [[[[ch0 b0 ]ofs0] v0] cp0]. destruct (j b0) as [[b0' ofs0'] |] eqn:JB.
+          + exploit mem_delta_apply_some. eapply APPD1. intros (mi1 & MEM1). rewrite MEM1 in APPD1.
+            exploit mem_delta_apply_inj_some. eapply APPD2. intros (mi2 & MEM2). rewrite MEM2 in APPD2.
+            simpl in *. eapply IHd. 3,4: eauto. 1,2: eapply Mem.perm_store_1; eauto.
+          + exploit mem_delta_apply_some. eapply APPD1. intros (mi1 & MEM1). rewrite MEM1 in APPD1. simpl in *. eapply IHd. 3,4: eauto. all: auto. eapply Mem.perm_store_1; eauto.
+        - exploit mem_delta_apply_some. eapply APPD1. intros (mi1 & MEM1). rewrite MEM1 in APPD1. destruct d0 as [[[w x] y] z]. simpl in *. eapply IHd. 3,4: eauto. all: auto.
+          eapply Mem.perm_storebytes_1; eauto.
+        - exploit mem_delta_apply_some. eapply APPD1. intros (mi1 & MEM1). rewrite MEM1 in APPD1. destruct d0 as [[x y] z]. simpl in *. eapply IHd. 3,4: eauto. all: auto.
+          destruct (Mem.alloc m1 x y z) eqn:ALLOC. simpl in MEM1. inv MEM1. eapply Mem.perm_alloc_1; eauto.
+        - exploit mem_delta_apply_some. eapply APPD1. intros (mi1 & MEM1). rewrite MEM1 in APPD1. destruct d0 as [[[w x] y] z]. simpl in *. eapply IHd. 3,4: eauto. all: auto.
+          eapply Mem.perm_free_1; eauto. left. intros CC. subst. congruence.
+    }
+    rename H into UNCHG. clear IHd. 
+    { destruct a.
+      - destruct d0 as [[[[ch0 b0] ofs0] v0] cp0]. destruct CHG as [CHG0 CHG1]. subst b0. rewrite INJ in APPD2.
+        exploit mem_delta_apply_some. eapply APPD1. intros (mi1 & MEM1). rewrite MEM1 in APPD1. exploit mem_delta_apply_inj_some. eapply APPD2. intros (mi2 & MEM2). rewrite MEM2 in APPD2.
+        simpl in *.
+        eapply mem_delta_unchanged_on in APPD1. exploit (Mem.unchanged_on_contents _ _ _ APPD1 b ofs); auto.
+        { eapply Mem.perm_store_1; eauto. }
+        intros. rewrite H; clear H.
+        eapply mem_delta_inj_unchanged_on in APPD2; auto. exploit (Mem.unchanged_on_contents _ _ _ APPD2 b' (ofs + ofsd)); auto.
+        { right. exists b, ofsd. split; auto. replace (ofs + ofsd - ofsd) with ofs by lia. auto. }
+        { eapply Mem.perm_store_1; eauto. }
+        intros. rewrite H; clear H.
+        eapply mem_store_same_upto_ofs; eauto.
+      - destruct d0 as [[[w x] y] z]. simpl in *. destruct CHG as [CHG0 CHG1]. subst w. rewrite WF1 in INJ. inv INJ.
+      - destruct d0 as [[x y] z]. simpl in *. inv CHG.
+      - destruct d0 as [[[w x] y] z]. simpl in *. inv CHG. rewrite WF1 in INJ. inv INJ.
+    }
+  Qed.
+
+  (* Lemma mem_delta_changed_only_by_store *)
+  (*       j d b ofs *)
+  (*       (INJ: j b <> None) *)
+  (*       (CHG: mem_delta_changed d b ofs) *)
+  (*       (WF: mem_delta_inj_wf j d) *)
+  (*   : *)
+  (*   mem_delta_changed_by_store_inj j d b ofs. *)
+  (* Proof. *)
+  (* Abort. *)
 
 
-(ZMap.get ofs (Mem.mem_contents m1) !! b1)
-Mem.store_mem_contents:
-  forall (chunk : memory_chunk) (m1 : mem) (b : block) (ofs : Z) (v : val) (cp : compartment) (m2 : mem),
-  Mem.store chunk m1 b ofs v cp = Some m2 -> Mem.mem_contents m2 = PMap.set b (Mem.setN (encode_val chunk v) ofs (Mem.mem_contents m1) !! b) (Mem.mem_contents m1)
-Mem.setN_in: forall (vl : list memval) (p q : Z) (c : ZMap.t memval), p <= q < p + Z.of_nat (Datatypes.length vl) -> In (ZMap.get q (Mem.setN vl p c)) vl
+  (* Lemma mem_delta_apply_store_preserves_winject *)
+  (*       (j: meminj) m0 m0' *)
+  (*       (WINJ0: winject j m0 m0') *)
+  (*       ch b ofs v cp *)
+  (*       m0 m1 *)
+  (*       (MEM: mem_delta_apply_store (Some m0) (ch, b, ofs, v, cp) = Some m1) *)
+  (*   : *)
+  (*   exists m1', mem_delta_apply_store_inj *)
+  (* exists m1' : mem, mem_delta_apply_inj j d (mem_delta_apply_store (Some m0') (ch, b', ofs + ofs', v, cp)) = Some m1' /\ winject j m1 m1' *)
 
+  Lemma mem_delta_apply_preserves_winject
+        (j: meminj) m0 m0'
+        (WINJ0: winject j m0 m0')
+        (d: mem_delta)
+        (DWF: mem_delta_inj_wf j d)
+        m1
+        (APPD: mem_delta_apply d (Some m0) = Some m1)
+    :
+    exists m1', (mem_delta_apply_inj j d (Some m0') = Some m1') /\ (winject j m1 m1').
+  Proof.
+    revert m0 m0' WINJ0 DWF m1 APPD. induction d; intros.
+    { inv APPD. simpl. exists m0'. split; auto. }
+    inv DWF. rename H1 into DWF1, H2 into DWF0. rewrite mem_delta_apply_cons in APPD. rewrite mem_delta_apply_inj_cons.
+    destruct a.
+    - destruct d0 as ((((ch & b) & ofs) & v) & cp). exploit mem_delta_apply_some. eauto. intros (mi & MEM). rewrite MEM in APPD.
+      destruct (j b) as [[b' ofs']|] eqn:JB.
+      + exploit store_mapped_winject; eauto. instantiate (1:=v). intros (mi0 & MEM' & WINJ1). specialize (IHd _ _ WINJ1 DWF0 _ APPD). destruct IHd as (m1' & APPD' & WINJ').
+        simpl in *. rewrite MEM'. eauto.
+      + exploit store_unmapped_winject; eauto.
+    - destruct d0 as (((b & ofs) & mvs) & cp). exploit mem_delta_apply_some. eauto. intros (mi & MEM). rewrite MEM in APPD. exploit storebytes_unmapped_winject; eauto.
+    - destruct d0 as ((cp & lo) & hi). exploit mem_delta_apply_some. eauto. intros (mi & MEM). rewrite MEM in APPD. simpl in *.
+      destruct (Mem.alloc m0 cp lo hi) eqn:ALLOC; simpl in *. inv MEM. exploit alloc_left_unmapped_winject_keep; eauto.
+    - destruct d0 as (((b & lo) & hi) & cp). exploit mem_delta_apply_some. eauto. intros (mi & MEM). rewrite MEM in APPD. exploit free_left_winject; eauto.
+  Qed.
 
+  Lemma mem_delta_apply_keeps_perm
+        j d
+        (DWF: mem_delta_inj_wf j d)
+        m0 m1
+        (APPD : mem_delta_apply d (Some m0) = Some m1)
+        b ofs
+        (INJ: j b <> None)
+        K P
+        (PERM: Mem.perm m1 b ofs K P)
+        (BOUND: (b < Mem.nextblock m0)%positive)
+    :
+    Mem.perm m0 b ofs K P.
+  Proof.
+    revert DWF m0 APPD BOUND. induction d; intros.
+    { simpl in *. inv APPD; auto. }
+    inv DWF. rename H1 into DWF1, H2 into DWF2. rewrite mem_delta_apply_cons in APPD. specialize (IHd DWF2).
+    destruct a; exploit mem_delta_apply_some; eauto; intros (mi & MEM); rewrite MEM in APPD; specialize (IHd _ APPD).
+    - destruct d0 as ((((ch0 & b0) & ofs0) & v0) & cp0). simpl in *. eapply Mem.perm_store_2; eauto. eapply IHd. erewrite Mem.nextblock_store; eauto.
+    - destruct d0 as (((b0 & ofs0) & mvs0) & cp0). simpl in *. eapply Mem.perm_storebytes_2; eauto. eapply IHd. erewrite Mem.nextblock_storebytes; eauto.
+    - destruct d0 as ((cp0 & lo0) & hi0). simpl in *. destruct (Mem.alloc m0 cp0 lo0 hi0) eqn:ALLOC. simpl in *. inv MEM.
+      exploit Mem.alloc_result; eauto. intros; subst b0. exploit Mem.nextblock_alloc; eauto. intros EQ.
+      eapply Mem.perm_alloc_4. eauto.  eapply IHd. lia. lia.
+    - destruct d0 as (((b0 & lo0) & hi0) & cp0). simpl in *.
+      eapply Mem.perm_free_3; eauto. eapply IHd. erewrite Mem.nextblock_free; eauto.
+  Qed.
 
+  Definition meminj_not_alloc (j: meminj) (m: mem) := forall b, (Mem.nextblock m <= b)%positive -> j b = None.
 
+  Lemma mem_delta_apply_establish_inject
+        (k j: meminj) m0 m0'
+        (INJ: Mem.inject k m0 m0')
+        (INCR: inject_incr j k)
+        (STRICT: meminj_strict j)
+        (NALLOC: meminj_not_alloc j m0)
+        (d: mem_delta)
+        (DWF: mem_delta_inj_wf j d)
+        m1
+        (APPD: mem_delta_apply d (Some m0) = Some m1)
+    :
+    exists m1', (mem_delta_apply_inj j d (Some m0') = Some m1') /\ (Mem.inject j m1 m1').
+  Proof.
+    exploit inject_implies_winject; eauto. intros WINJ. exploit winject_inj_incr; eauto. clear WINJ; intro WINJ.
+    exploit mem_delta_apply_preserves_winject; eauto. intros (m1' & APPD' & WINJ'). exists m1'. split; auto.
+    apply winject_to_inject; auto. unfold mem_inj_val. intros.
+    exploit mem_delta_apply_keeps_perm; eauto. congruence.
+    { destruct (Pos.ltb_spec0 b1 (Mem.nextblock m0)); auto. exfalso. assert (j b1 = None).
+      { eapply NALLOC. lia. }
+      congruence.
+    }
+    intros PERM0.
+    destruct (mem_delta_unchanged_or_changed d b1 ofs).
+    - exploit mem_delta_unchanged_on; eauto. intros UNCHG1. exploit mem_delta_inj_unchanged_on; eauto. intros UNCHG2.
+      erewrite (Mem.unchanged_on_contents _ _ _ UNCHG1). erewrite (Mem.unchanged_on_contents _ _ _ UNCHG2). all: eauto.
+      2:{ right. exists b1, delta. split; auto. replace (ofs + delta - delta) with ofs by lia. auto. }
+      { inv INJ. inv mi_inj. eapply mi_memval.
+        (* TODO *)
+      
+      { clear - INJ INCR 
 
-
-
-Mem.store_mem_contents:
-  forall (chunk : memory_chunk) (m1 : mem) (b : block) (ofs : Z) (v : val) (cp : compartment) (m2 : mem),
-  Mem.store chunk m1 b ofs v cp = Some m2 -> Mem.mem_contents m2 = PMap.set b (Mem.setN (encode_val chunk v) ofs (Mem.mem_contents m1) !! b) (Mem.mem_contents m1)
-Mem.storebytes_mem_contents:
-  forall (m1 : mem) (b : block) (ofs : Z) (bytes : list memval) (cp : compartment) (m2 : mem),
-  Mem.storebytes m1 b ofs bytes cp = Some m2 -> Mem.mem_contents m2 = PMap.set b (Mem.setN bytes ofs (Mem.mem_contents m1) !! b) (Mem.mem_contents m1)
-
-
-
-
-  Mem.unchanged_on_contents:
+      
+      eauto
+      .unchanged_on_contents:
   forall (P : block -> Z -> Prop) (m_before m_after : mem),
   Mem.unchanged_on P m_before m_after ->
   forall (b : block) (ofs : Z), P b ofs -> Mem.perm m_before b ofs Cur Readable -> ZMap.get ofs (Mem.mem_contents m_after) !! b = ZMap.get ofs (Mem.mem_contents m_before) !! b
-
-    mi_memval : forall (b1 : block) (ofs : Z) (b2 : block) (delta : Z),
-                f b1 = Some (b2, delta) -> Mem.perm m1 b1 ofs Cur Readable -> memval_inject f (ZMap.get ofs (Mem.mem_contents m1) !! b1) (ZMap.get (ofs + delta) (Mem.mem_contents m2) !! b2) }.
-
-
-Mem.load_store_overlap:
-  forall (chunk : memory_chunk) (m1 : mem) (b : block) (ofs : Z) (v : val) (cp : compartment) (m2 : mem) (chunk' : memory_chunk) (ofs' : Z) (cp' : option compartment) (v' : val),
-  Mem.store chunk m1 b ofs v cp = Some m2 ->
-  Mem.load chunk' m2 b ofs' cp' = Some v' ->
-  ofs' + size_chunk chunk' > ofs ->
-  ofs + size_chunk chunk > ofs' ->
-  exists (mv1 : memval) (mvl : list memval) (mv1' : memval) (mvl' : list memval),
-    shape_encoding chunk v (mv1 :: mvl) /\ shape_decoding chunk' (mv1' :: mvl') v' /\ (ofs' = ofs /\ mv1' = mv1 \/ ofs' > ofs /\ In mv1' mvl \/ ofs' < ofs /\ In mv1 mvl')
-
-
-
-  (* Properties *)
-  Lemma alloc_left_unmapped_winject_keep:
-    forall f m1 m2 c lo hi m1' b1,
-      winject f m1 m2 ->
-      Mem.alloc m1 c lo hi = (m1', b1) ->
-      winject f m1' m2.
+        
+        (d_pre d_post: mem_delta)
+        (DWFPRE: mem_delta_inj_wf j d_pre)
+        (DWFPOST: mem_delta_inj_wf j d_post)
+        m_m
+        (APPDPRE: mem_delta_apply_left d_pre (Some m_i) = Some m_m)
+        (WINJ: mem_weak_inject j m_m m0')
+        m_f
+        (APPDPOST: mem_delta_apply_left d_post (Some m_m) = Some m_f)
+        (MFO: meminj_first_order j m_f)
+    :
+    exists m1', (mem_delta_apply_inj j (d_pre ++ d_post) m0' = Some m1') /\ (Mem.inject j m_f m1').
   Proof.
-    intros. set (f' := fun b => if eq_block b b1 then None else f b).
-    cut (winject f' m1' m2 /\ inject_incr f f' /\ f' b1 = None /\ (forall b, b <> b1 -> f' b = f b)).
-    { clear - f'. intros (INJ & INCR & _ & _). unfold inject_incr in INCR.
-      assert (f' = f).
-      { eapply Axioms.functional_extensionality. intros x. destruct (eq_block x b1).
-        - subst x. destruct (f b1) eqn:FB.
-          + destruct p. specialize (INCR _ _ _ FB). auto.
-          + subst f'. simpl. rewrite pred_dec_true; auto.
-        - subst f'. simpl. rewrite pred_dec_false; auto.
-      }
-      rewrite <- H. apply INJ.
-    }
-    inversion H. assert (inject_incr f f').
-    red; unfold f'; intros. destruct (eq_block b b1). subst b.
-    assert (f b1 = None). eauto with mem. congruence.
-    auto.
-    assert (mem_winj f' m1 m2).
-    inversion mwi_inj; constructor; eauto with mem.
-    unfold f'; intros. destruct (eq_block b0 b1). congruence. eauto.
-    unfold f'; intros. destruct (eq_block b0 b1). congruence. eauto.
-    unfold f'; intros. destruct (eq_block b0 b1). congruence.
-    unfold f'; intros. destruct (eq_block b0 b1). congruence.
-    eapply mwi_align; eauto.
-    split. constructor.
-    (* inj *)
-    eapply alloc_left_unmapped_winj; eauto. unfold f'; apply dec_eq_true.
-    (* freeblocks *)
-    intros. unfold f'. destruct (eq_block b b1). auto.
-    apply mi_freeblocks. red; intro; elim H3. eauto with mem.
-    (* mappedblocks *)
-    unfold f'; intros. destruct (eq_block b b1). congruence. eauto.
-    (* no overlap *)
-    unfold f'; red; intros.
-    destruct (eq_block b0 b1); destruct (eq_block b2 b1); try congruence.
-    eapply mwi_no_overlap. eexact H3. eauto. eauto.
-    exploit Mem.perm_alloc_inv. eauto. eexact H6. rewrite dec_eq_false; auto.
-    exploit Mem.perm_alloc_inv. eauto. eexact H7. rewrite dec_eq_false; auto.
-    (* representable *)
-    unfold f'; intros.
-    destruct (eq_block b b1); try discriminate.
-    eapply mwi_representable; try eassumption.
-    destruct H4; eauto using Mem.perm_alloc_4.
-    (* perm inv *)
-    intros. unfold f' in H3; destruct (eq_block b0 b1); try discriminate.
-    exploit mwi_perm_inv; eauto.
-    intuition eauto using Mem.perm_alloc_1, Mem.perm_alloc_4.
-    (* incr *)
-    split. auto.
-    (* image *)
-    split. unfold f'; apply dec_eq_true.
-    (* incr *)
-    intros; unfold f'; apply dec_eq_false; auto.
-  Qed.
 
-  Lemma alloc_left_unmapped_inject_keep:
-    forall f m1 m2 c lo hi m1' b1,
-      Mem.inject f m1 m2 ->
-      Mem.alloc m1 c lo hi = (m1', b1) ->
-      Mem.inject f m1' m2.
-  Proof.
-    intros. set (f' := fun b => if eq_block b b1 then None else f b).
-    cut (Mem.inject f' m1' m2 /\ inject_incr f f' /\ f' b1 = None /\ (forall b, b <> b1 -> f' b = f b)).
-    { clear - f'. intros (INJ & INCR & _ & _). unfold inject_incr in INCR.
-      assert (f' = f).
-      { eapply Axioms.functional_extensionality. intros x. destruct (eq_block x b1).
-        - subst x. destruct (f b1) eqn:FB.
-          + destruct p. specialize (INCR _ _ _ FB). auto.
-          + subst f'. simpl. rewrite pred_dec_true; auto.
-        - subst f'. simpl. rewrite pred_dec_false; auto.
-      }
-      rewrite <- H. apply INJ.
-    }
-    inversion H. assert (inject_incr f f').
-    red; unfold f'; intros. destruct (eq_block b b1). subst b.
-    assert (f b1 = None). eauto with mem. congruence.
-    auto.
-    assert (Mem.mem_inj f' m1 m2).
-    inversion mi_inj; constructor; eauto with mem.
-    unfold f'; intros. destruct (eq_block b0 b1). congruence. eauto.
-    unfold f'; intros. destruct (eq_block b0 b1). congruence. eauto.
-    unfold f'; intros. destruct (eq_block b0 b1). congruence.
-    unfold f'; intros. destruct (eq_block b0 b1). congruence.
-    eapply mi_align; eauto.
-    unfold f'; intros. destruct (eq_block b0 b1). congruence.
-    apply memval_inject_incr with f; auto.
-    split. constructor.
-    (* inj *)
-    eapply Mem.alloc_left_unmapped_inj; eauto. unfold f'; apply dec_eq_true.
-    (* freeblocks *)
-    intros. unfold f'. destruct (eq_block b b1). auto.
-    apply mi_freeblocks. red; intro; elim H3. eauto with mem.
-    (* mappedblocks *)
-    unfold f'; intros. destruct (eq_block b b1). congruence. eauto.
-    (* no overlap *)
-    unfold f'; red; intros.
-    destruct (eq_block b0 b1); destruct (eq_block b2 b1); try congruence.
-    eapply mi_no_overlap. eexact H3. eauto. eauto.
-    exploit Mem.perm_alloc_inv. eauto. eexact H6. rewrite dec_eq_false; auto.
-    exploit Mem.perm_alloc_inv. eauto. eexact H7. rewrite dec_eq_false; auto.
-    (* representable *)
-    unfold f'; intros.
-    destruct (eq_block b b1); try discriminate.
-    eapply mi_representable; try eassumption.
-    destruct H4; eauto using Mem.perm_alloc_4.
-    (* perm inv *)
-    intros. unfold f' in H3; destruct (eq_block b0 b1); try discriminate.
-    exploit mi_perm_inv; eauto.
-    intuition eauto using Mem.perm_alloc_1, Mem.perm_alloc_4.
-    (* incr *)
-    split. auto.
-    (* image *)
-    split. unfold f'; apply dec_eq_true.
-    (* incr *)
-    intros; unfold f'; apply dec_eq_false; auto.
-  Qed.
+
+  (* TODO *)
 
   Lemma mem_delta_apply_preserves_full
         (k j: meminj) m_i m0'
@@ -682,7 +941,6 @@ Mem.load_store_overlap:
     :
     exists m1', (mem_delta_apply_inj j (d_pre ++ d_post) m0' = Some m1') /\ (Mem.inject j m_f m1').
   Proof.
-
 
 
     rewrite mem_delta_apply_eq in APPD. rewrite mem_delta_apply_inj_eq. rewrite mem_delta_inj_wf_rev in DWF. remember (rev d) as rd. clear d Heqrd. rename rd into d.
@@ -724,6 +982,10 @@ Mem.load_store_overlap:
     - destruct d0 as (((b & lo) & hi) & cp). simpl in *.
       exists m_i'; split; auto. eapply Mem.free_left_inject; eauto.
   Qed.
+
+
+
+
 
   Lemma val_inject_incr_inv
         f f' v v'
@@ -893,12 +1155,6 @@ Mem.store_mem_contents:
       exists m_i'; split; auto. eapply Mem.free_left_inject; eauto.
   Qed.
 
-  (* Memory injection for public global symbols: visible for external calls *)
-  Definition meminj_public (ge: Senv.t): meminj :=
-    fun b => match Senv.invert_symbol ge b with
-          | Some id => if Senv.public_symbol ge id then Some (b, 0%Z) else None
-          | None => None
-          end.
 
 
         (DFO: mem_delta_inj_fo j d)
